# baseURI: http://duraark.eu/vocabularies/ifcm
# imports: http://bloody-byte.net/rdf/dc_owl2dl/dcmitype.ttl
# imports: http://purl.org/dc/terms/
# imports: http://www.loc.gov/premis/rdf/v1
# imports: http://www.w3.org/2004/02/skos/core
# imports: http://www.w3.org/TR/prov-o/

@prefix : <http://duraark.eu/vocabularies/ifcm#> .
@prefix owl: <http://www.w3.org/2002/07/owl#> .
@prefix premisowl: <http://www.loc.gov/premis/rdf/v1#> .
@prefix provo: <http://www.w3.org/TR/prov-o#> .
@prefix rdf: <http://www.w3.org/1999/02/22-rdf-syntax-ns#> .
@prefix rdfs: <http://www.w3.org/2000/01/rdf-schema#> .
@prefix skos: <http://www.w3.org/2004/02/skos/core#> .
@prefix xsd: <http://www.w3.org/2001/XMLSchema#> .

<http://duraark.eu/vocabularies/ifcm>
	rdf:type owl:Ontology ;
	owl:imports <http://bloody-byte.net/rdf/dc_owl2dl/dcmitype.ttl> ,
		<http://www.w3.org/TR/prov-o/> , <http://www.w3.org/2004/02/skos/core> ,
		<http://purl.org/dc/terms/> , <http://www.loc.gov/premis/rdf/v1> ;
	owl:versionInfo "Initital draft M12"^^xsd:string .
	
:IFCCharacteristics
	rdf:type owl:Class ;
	rdfs:comment "A domain specific PREMIS ObjectCharacteristics extension that
		describes File entities of the Industry Foundation Classes in their part
		21 STEP Physical File Format (SPFF)"^^xsd:string ;
	rdfs:label "IFC Characteristics"^^xsd:string ;
	rdfs:subClassOf premisowl:ObjectCharacteristicsExtension ;
	skos:prefLabel "IFC Characteristics"^^xsd:string .
	
:LODmetric
	rdf:type owl:DatatypeProperty ;
	rdfs:comment "a percentage ratio that determines the number of object per
		quibical meter"^^xsd:string ;
	rdfs:label "LODmetric"^^xsd:string ;
	rdfs:range xsd:float .
	
:attributeMetric
	rdf:type owl:DatatypeProperty ;
	rdfs:comment "the percentage of the OPTIONAL schema-level attributes that
		have are provied with values in this file"^^xsd:string ;
	rdfs:domain :IFCCharacteristics ;
	rdfs:label "attribute metric"^^xsd:string ;
	rdfs:range xsd:float .
	
:componentLibaries
	rdf:type owl:DatatypeProperty ;
	rdfs:comment "name of external component library that has been used. Can be
		instantiated multiple times"^^xsd:string ;
	rdfs:domain :IFCCharacteristics ;
	rdfs:label "component libaries"^^xsd:string ;
	rdfs:range xsd:string .
	
:creationTime
	rdf:type owl:DatatypeProperty ;
	rdfs:comment "timestamp of the generation of this file from the header
		"^^xsd:string ;
	rdfs:label "creation time"^^xsd:string ;
	rdfs:range xsd:dateTime .
	
:ifcVersion
	rdf:type owl:DatatypeProperty ;
	rdfs:comment "The version of the IFC file. Can be extracted from the header
		e.g. FILE_SCHEMA ((’IFC2X3’)). Will be IFC2x3 most of the times by the
	time of this initial version"^^xsd:string ;
	rdfs:domain :IFCCharacteristics ;
	rdfs:label "has IFC version"^^xsd:string ;
	rdfs:range xsd:string .
	
:implemenationLevel
	rdf:type owl:DatatypeProperty ;
	rdfs:comment "The implementation level according to the ISO 10303:21, most
		often this will be ’2;1’"^^xsd:string ;
	rdfs:domain :IFCCharacteristics ;
	rdfs:label "implemenation level"^^xsd:string ;
	rdfs:range xsd:string .
	
:lastProducingApplication
	rdf:type owl:ObjectProperty ;
	rdfs:comment "the LAST Software application that has been involved in
		creating this model. In contrast to teh producingApplication property,
		this information should be taken from the header"^^xsd:string ;
	rdfs:domain :IFCCharacteristics ;
	rdfs:label "originating application"^^xsd:string ;
	rdfs:range <http://purl.org/dc/dcmitype/Software> .
	
:mvd rdf:type owl:DatatypeProperty ;
	rdfs:comment "the Model View Definition this file complies to. Can be
		extracted from the FILE_DESCRIPTION section in the SPFF
	header"^^xsd:string ;
	rdfs:label "has MVD"^^xsd:string ;
	rdfs:range xsd:string .
	
:numberComponents
	rdf:type owl:DatatypeProperty ;
	rdfs:comment "The number of IfcProduct subtypes that have been instantiated
		(doors, windows, roofs, walls etc)"^^xsd:string ;
	rdfs:domain :IFCCharacteristics ;
	rdfs:label "number or products"^^xsd:string ;
	rdfs:range xsd:integer .

:numberEntities
	rdf:type owl:DatatypeProperty ;
	rdfs:comment ""^^xsd:string ;
	rdfs:domain :IFCCharacteristics ;
	rdfs:label "number entities"^^xsd:string ;
	rdfs:range xsd:integer .
	
:producingApplication
	rdf:type owl:ObjectProperty ;
	rdfs:comment "one of the software application that has been involved in
		creating this model. This information can be extracted on a per-object
		record from the asscociated IfcOwnerHistory record. In theory. In
		practice this provenance metadata record is not used to its intended
		purpose in most implementing applications."^^xsd:string ;
	rdfs:domain :IFCCharacteristics ;
	rdfs:label "producing Application"^^xsd:string ;
	rdfs:range <http://purl.org/dc/dcmitype/Software> .
	
premisowl:ObjectCharacteristicsExtension
	rdf:type owl:Class ;
	rdfs:comment "A Container Class to implement domain-specific
		extensions"^^xsd:string ;
	rdfs:label "Object characteristics extension"^^xsd:string ;
	rdfs:subClassOf premisowl:ObjectCharacteristics ;
	skos:prefLabel "Object characteristics extension"^^xsd:string .
	
	